CakeML-friendly exec sem parameterised over native word size, exec sem parameterised over uninitialised variable handling

hol/cake_sem/p4_cake_auxLib.sig
@@ -2,6 +2,8 @@ signature p4_cake_auxLib =
 sig
   include Abbrev
 
+val native_word : hol_type
+
 val BOOL_LIST_ss : simpLib.ssfrag
 
 val BOOL_LIST_ss' : simpLib.ssfrag
